done with soundness of memory

memory_cmp_impl.v
@@ -102,17 +102,6 @@ Module MemoryCmpImpl.
         | _, _ => false
         end
     end.
-
-  (*
-  Definition swap_memory_update (u1 u2 : memory_update sstack_val) : bool :=
-    match u1, u2 with
-    | U_MSTORE _ (Val v1) _, U_MSTORE _ (Val v2) _ => ((wordToN v2)+31 <? (wordToN v1))%N
-    | U_MSTORE8 _ (Val v1) _, U_MSTORE8 _ (Val v2) _ => ((wordToN v2) <? (wordToN v1))%N
-    | U_MSTORE _ (Val v1) _, U_MSTORE8 _ (Val v2) _ => ((wordToN v2) <? (wordToN v1))%N
-    | U_MSTORE8 _ (Val v1) _, U_MSTORE _ (Val v2) _ => ((wordToN v2)+31 <? (wordToN v1))%N
-    | _,_ => false                                                             
-    end.
-   *)
   
   Fixpoint reorder_updates' (d : nat) (smem :smemory) (maxidx: nat) (sb: sbindings) : bool * smemory :=
     match d with
